src/cpp2v.cpp
@@ -61,6 +61,11 @@ static cl::opt<bool>
 static cl::opt<bool> Version("cpp2v-version", cl::Optional, cl::ValueOptional,
                              cl::cat(Cpp2V));
 
+static cl::opt<bool>
+    Templates("templates",
+        cl::desc("generate AST for templated code"),
+        cl::cat(Cpp2V));
+
 class ToCoqAction : public clang::ASTFrontendAction {
 public:
     virtual std::unique_ptr<clang::ASTConsumer>
@@ -73,8 +78,8 @@ public:
             llvm::errs() << i << "\n";
         }
 #endif
-        auto result = new ToCoqConsumer(&Compiler, to_opt(VFileOutput),
-                                        to_opt(NamesFile));
+        auto result = new ToCoqConsumer(&Compiler, Templates,
+            to_opt(VFileOutput), to_opt(NamesFile));
         return std::unique_ptr<clang::ASTConsumer>(result);
     }
 
