theories/lang/cpp/semantics/types.v
@@ -74,6 +74,8 @@ Fixpoint size_of (resolve : genv) (t : type) : option N :=
   | Tnullptr => Some (pointer_size resolve)
   | Tfloat sz => Some (bytesN sz)
   | Tarch sz _ => bytesN <$> sz
+  | Tvar _
+  | Tdependent => None
   end%N.
 
 #[global] Instance Proper_size_of
